src/ExprTac.v
@@ -8,18 +8,9 @@ Section abstracted.
             (funcs : functions types)
             (meta_env var_env : env types).
 
-  Fixpoint nexprD (e : expr types) (t : tvar) {struct e} : 
+  Fixpoint nexprD (e : expr) (t : tvar) {struct e} : 
     option (tvarD types t) :=
     match e with
-      | Const t' c =>
-        match equiv_dec t' t with
-          | left pf =>
-            Some
-            match pf in (_ = t0) return (tvarD types t0) with
-              | eq_refl => c
-            end
-          | right _ => None
-        end
       | Var x => lookupAs var_env t x
       | Func f xs =>
         match nth_error funcs f with
@@ -28,7 +19,7 @@ Section abstracted.
               | left pf =>
                 match pf in (_ = t0) return (option (tvarD types t0)) with
                   | eq_refl =>
-                    applyD nexprD (Domain f0) xs (tvarD types (Range f0))
+                    applyD types nexprD (Domain f0) xs (tvarD types (Range f0))
                     (Denotation f0)
                 end
               | right _ => None
@@ -60,7 +51,7 @@ Section abstracted.
       | UVar x => lookupAs meta_env t x
     end.
 
-  Fixpoint nAllProvable_impl (k : Prop) (es : list (expr types)) : Prop :=
+  Fixpoint nAllProvable_impl (k : Prop) (es : list expr) : Prop :=
     match es with
       | nil => k
       | e :: es =>
@@ -70,7 +61,7 @@ Section abstracted.
         end -> nAllProvable_impl k es
     end.
 
-  Fixpoint nAllProvable_and (k : Prop) (es : list (expr types)) : Prop :=
+  Fixpoint nAllProvable_and (k : Prop) (es : list expr) : Prop :=
     match es with
       | nil => k
       | e :: es =>
