src/ExprUnify.v
@@ -9,13 +9,13 @@ Module Type SemanticUnifier (S : Subst).
     Variable types : list type.
 
     (** The actual unification algorithm **)
-    Parameter exprUnify : nat -> expr types -> expr types -> S.Subst types -> option (S.Subst types).
+    Parameter exprUnify : nat -> expr -> expr -> S.Subst -> option S.Subst.
 
     (** This is the soundness statement. **)
     Axiom exprUnify_sound_sem : forall n l r sub sub',
       exprUnify n l r sub = Some sub' ->
       forall funcs U G t,
-      exprD funcs U G (S.exprInstantiate sub' l) t = 
+      exprD (types := types) funcs U G (S.exprInstantiate sub' l) t = 
       exprD funcs U G (S.exprInstantiate sub' r) t.
 
     Axiom exprUnify_Extends : forall n l r sub sub',
@@ -41,7 +41,7 @@ Module Type SyntacticUnifier (S : Subst).
 
     (** This is the soundness statement. **)
     Axiom exprUnify_sound_syn : forall n l r sub sub',
-      @exprUnify types n l r sub = Some sub' ->
+      @exprUnify n l r sub = Some sub' ->
       S.exprInstantiate sub' l = S.exprInstantiate sub' r.
        
   End typed.
@@ -52,7 +52,7 @@ Module SyntacticKernel (S : Subst).
     Variable types : list type.
 
     (** The actual unification algorithm **)
-    Parameter exprUnify : nat -> expr types -> expr types -> S.Subst types -> option (S.Subst types).
+    Parameter exprUnify : nat -> expr -> expr -> S.Subst -> option S.Subst.
 
     (** This is the soundness statement. **)
     Axiom exprUnify_sound_syn : forall n l r sub sub',
